rustfrontend/RustIRgen.v
@@ -7,246 +7,14 @@ Require Import Values.
 Require Import AST.
 Require Import Ctypes Rusttypes.
 Require Import Cop.
-Require Import RustlightBase RustIR.
+Require Import RustlightBase Selector.
 
 
-(** Translation from Rustlight to RustIR. The first step is
-translating the AST style program into CFG style program which is
-useful for analyzing. The second step is to generate the drop
-operation based on the ownership semantics in the source program. *)
+(** Translation from Rustlight to RustIR. The main step is to generate
+the drop operations and lifetime annotations in the end of a
+variable. We also need to insert drops for those out-of-scope variable
+in [break] and [continue] *)
 
-(** * Translation state *)
-
-Record state: Type := mkstate {
-  st_nextnode: node;
-  st_code: code;
-  st_wf: forall (pc: node), Plt pc st_nextnode \/ st_code!pc = None
-}.
-
-
-Inductive state_incr: state -> state -> Prop :=
-  state_incr_intro:
-    forall (s1 s2: state),
-    Ple s1.(st_nextnode) s2.(st_nextnode) ->
-    (forall pc,
-        s1.(st_code)!pc = None \/ s2.(st_code)!pc = s1.(st_code)!pc) ->
-    state_incr s1 s2.
-
-Lemma state_incr_refl:
-  forall s, state_incr s s.
-Proof.
-  intros. apply state_incr_intro.
-  apply Ple_refl.
-  intros. auto.
-Qed.
-
-Lemma state_incr_trans:
-  forall s1 s2 s3, state_incr s1 s2 -> state_incr s2 s3 -> state_incr s1 s3.
-Proof.
-  intros. inv H; inv H0. apply state_incr_intro.
-  apply Ple_trans with (st_nextnode s2); assumption.
-  intros. generalize (H2 pc) (H3 pc). intuition congruence.
-Qed.
-
-(** ** The state and error monad *)
-
-(* just copy from RTLgen *)
-
-Inductive res (A: Type) (s: state): Type :=
-  | Error: Errors.errmsg -> res A s
-  | OK: A -> forall (s': state), state_incr s s' -> res A s.
-
-Arguments OK [A s].
-Arguments Error [A s].
-
-Definition mon (A: Type) : Type := forall (s: state), res A s.
-
-Definition ret {A: Type} (x: A) : mon A :=
-  fun (s: state) => OK x s (state_incr_refl s).
-
-
-Definition error {A: Type} (msg: Errors.errmsg) : mon A := fun (s: state) => Error msg.
-
-Definition bind {A B: Type} (f: mon A) (g: A -> mon B) : mon B :=
-  fun (s: state) =>
-    match f s with
-    | Error msg => Error msg
-    | OK a s' i =>
-        match g a s' with
-        | Error msg => Error msg
-        | OK b s'' i' => OK b s'' (state_incr_trans s s' s'' i i')
-        end
-    end.
-
-Definition bind2 {A B C: Type} (f: mon (A * B)) (g: A -> B -> mon C) : mon C :=
-  bind f (fun xy => g (fst xy) (snd xy)).
-
-Notation "'do' X <- A ; B" := (bind A (fun X => B))
-   (at level 200, X ident, A at level 100, B at level 200).
-Notation "'do' ( X , Y ) <- A ; B" := (bind2 A (fun X Y => B))
-   (at level 200, X ident, Y ident, A at level 100, B at level 200).
-
-Definition handle_error {A: Type} (f g: mon A) : mon A :=
-  fun (s: state) =>
-    match f s with
-    | OK a s' i => OK a s' i
-    | Error _ => g s
-    end.
-
-(** Move path environment: a map from places (move path) to temporary variables  *)
-
-Record move_path_env := {
-    move_map: PTree.t (list (place * ident))
-  }.
-
-Definition move_path_index (me: move_path_env) (p: place) : option ident :=
-  match me.(move_map) ! (local_of_place p) with
-  | Some l =>
-      match filter (fun elt => if place_eq (fst elt) p then true else false) l with
-      | nil => None
-      | (_,id) :: _ => Some id
-      end
-  | None => None
-  end.
-
-
-
-(** ** Operations on state *)
-
-(** The initial state (empty CFG). *)
-
-Remark init_state_wf:
-  forall pc, Plt pc 1%positive \/ (PTree.empty statement)!pc = None.
-Proof. intros; right; apply PTree.gempty. Qed.
-
-Definition init_state : state :=
-  mkstate 1%positive (PTree.empty statement) init_state_wf.
-
-
-Remark add_instr_wf:
-  forall s i pc,
-  let n := s.(st_nextnode) in
-  Plt pc (Pos.succ n) \/ (PTree.set n i s.(st_code))!pc = None.
-Proof.
-  intros. case (peq pc n); intro.
-  subst pc; left; apply Plt_succ.
-  rewrite PTree.gso; auto.
-  elim (st_wf s pc); intro.
-  left. apply Plt_trans_succ. exact H.
-  right; assumption.
-Qed.
-
-Remark add_instr_incr:
-  forall s i,
-  let n := s.(st_nextnode) in
-  state_incr s (mkstate (Pos.succ n)
-                  (PTree.set n i s.(st_code))
-                  (add_instr_wf s i)).
-Proof.
-  constructor; simpl.
-  apply Ple_succ.
-  intros. destruct (st_wf s pc). right. apply PTree.gso. apply Plt_ne; auto. auto.
-Qed.
-
-Definition add_instr (i: statement) : mon node :=
-  fun s =>
-    let n := s.(st_nextnode) in
-    OK n
-       (mkstate (Pos.succ n) (PTree.set n i s.(st_code))
-                (add_instr_wf s i))
-       (add_instr_incr s i).
-
-(** [add_instr] can be decomposed in two steps: reserving a fresh
-  CFG node, and filling it later with an instruction.  This is needed
-  to compile loops. *)
-
-Remark reserve_instr_wf:
-  forall s pc,
-  Plt pc (Pos.succ s.(st_nextnode)) \/ s.(st_code)!pc = None.
-Proof.
-  intros. elim (st_wf s pc); intro.
-  left; apply Plt_trans_succ; auto.
-  right; auto.
-Qed.
-
-Remark reserve_instr_incr:
-  forall s,
-  let n := s.(st_nextnode) in
-  state_incr s (mkstate (Pos.succ n)
-                  s.(st_code)
-                      (reserve_instr_wf s)).
-Proof.
-  intros; constructor; simpl.
-  apply Ple_succ.
-  auto.
-Qed.
-
-Definition reserve_instr: mon node :=
-  fun (s: state) =>
-  let n := s.(st_nextnode) in
-  OK n
-     (mkstate (Pos.succ n) s.(st_code) (reserve_instr_wf s))
-     (reserve_instr_incr s).
-
-Remark update_instr_wf:
-  forall s n i,
-  Plt n s.(st_nextnode) ->
-  forall pc,
-  Plt pc s.(st_nextnode) \/ (PTree.set n i s.(st_code))!pc = None.
-Proof.
-  intros.
-  case (peq pc n); intro.
-  subst pc; left; assumption.
-  rewrite PTree.gso; auto. exact (st_wf s pc).
-Qed.
-
-Remark update_instr_incr:
-  forall s n i (LT: Plt n s.(st_nextnode)),
-  s.(st_code)!n = None ->
-  state_incr s
-             (mkstate s.(st_nextnode) (PTree.set n i s.(st_code))
-                     (update_instr_wf s n i LT)).
-Proof.
-  intros.
-  constructor; simpl; intros.
-  apply Ple_refl.
-  rewrite PTree.gsspec. destruct (peq pc n). left; congruence. right; auto.
-Qed.
-
-Definition check_empty_node:
-  forall (s: state) (n: node), { s.(st_code)!n = None } + { True }.
-Proof.
-  intros. case (s.(st_code)!n); intros. right; auto. left; auto.
-Defined.
-
-Definition update_instr (n: node) (i: statement) : mon unit :=
-  fun s =>
-    match plt n s.(st_nextnode), check_empty_node s n with
-    | left LT, left EMPTY =>
-        OK tt
-           (mkstate s.(st_nextnode) (PTree.set n i s.(st_code))
-                    (update_instr_wf s n i LT))
-           (update_instr_incr s n i LT EMPTY)
-    | _, _ =>
-        Error (Errors.msg "RTLgen.update_instr")
-    end.             
-
-(* add drop statement *)
-Definition add_drop (ce: composite_env) (p: place) (succ: node) : mon node :=
-  match own_type own_fuel ce (typeof_place p) with
-  | Some true => add_instr (Sdrop p succ)
-  | Some false => ret succ
-  | None => error (Errors.msg "Running out of fuel in own_type in add_drop.")
-  end.
-
-Definition add_instr_endscope (ce: composite_env) (local: ident) (ty: type) (succ: node): mon node :=
-  do n1 <- add_instr (Sstoragedead local succ);
-  do n2 <- add_drop ce (Plocal local ty) n1;
-  ret n2.
-
-(* when a list of locals go out of scope, add [Drop] and [Sstoragedead] for them *)
-Definition add_endscope_list (ce: composite_env) (locals: list (ident * type)) (succ: node) : mon node :=
-  fold_right (fun elt acc => do n <- acc; add_instr_endscope ce (fst elt) (snd elt) n) (ret succ) locals.
 
 Definition list_list_cons {A: Type} (e: A) (l: list (list A)) :=
   match l with
@@ -254,143 +22,89 @@ Definition list_list_cons {A: Type} (e: A) (l: list (list A)) :=
   | l' :: l => (e::l') :: l
   end.
 
-(** Translation of statement *)
+Fixpoint makeseq_rec (s: statement) (l: list statement) : statement :=
+  match l with
+  | nil => s
+  | s' :: l' => makeseq_rec (Ssequence s s') l'
+  end.
 
-Section COMPOSITE_ENV.
+Definition makeseq (l: list statement) : statement :=
+  makeseq_rec Sskip l.
 
-Variable (ce: composite_env).
+Definition gen_drops (l: list (ident * type)) : statement :=
+  let drops := map (fun elt => (Sdrop (Plocal (fst elt) (snd elt)))) l in
+  makeseq drops.
 
-Fixpoint transl_stmt (stmt: RustlightBase.statement) (succ: node) (live_vars: list (list (ident * type))) (cont: option node) (break: option node) {struct stmt} : mon node :=
-    match stmt with
-    | RustlightBase.Sskip =>
-        add_instr (Sskip succ)
-    | Slet id ty e stmt' =>
-        do n1 <- add_instr_endscope ce id ty succ;
-        do n2 <- transl_stmt stmt' n1 (list_list_cons (id,ty) live_vars) cont break;
-        do n3 <- add_instr (Sassign (Plocal id ty) e n2);
-        do n4 <- add_instr (Sstoragelive id n3);
-        ret n4
-    | RustlightBase.Sassign p e =>
-        do n1 <- add_drop ce p succ;
-        do n2 <- add_instr (Sassign p e n1);
-        ret n2
-    | Ssequence stmt1 stmt2 =>
-        do succ2 <- transl_stmt stmt2 succ live_vars cont break;
-        do succ1 <- transl_stmt stmt1 succ2 live_vars cont break;
-        ret succ1
-    | RustlightBase.Sifthenelse e stmt1 stmt2 =>
-        do n1 <- transl_stmt stmt1 succ live_vars cont break;
-        do n2 <- transl_stmt stmt2 succ live_vars cont break;
-        do n3 <- add_instr (Sifthenelse e n1 n2);
-        ret n3
-    | Sloop stmt =>
-        do loop_start <- reserve_instr;
-        do body_start <- transl_stmt stmt succ (nil::live_vars) (Some loop_start) (Some succ);
-        do _ <- update_instr loop_start (Sskip body_start);
-        ret loop_start
-    | Sbreak =>
-        match break with
-        | None =>
-            error (Errors.msg "No loop outside the break")
-        | Some brk =>
-            match live_vars with
-            | nil =>             (* nothing to drop *)
-                do succ' <- add_instr (Sskip brk);
-                ret succ'
-            | locals :: _ =>
-                do drop_start <- add_endscope_list ce locals brk;
-                do succ' <- add_instr (Sskip drop_start);
-                ret succ'
-            end
-        end
-    | Scontinue =>
-        match cont with
-        | None =>
-            error (Errors.msg "No loop outside the continue")
-        | Some cont =>            
-            match live_vars with
-            | nil =>
-                do succ' <- add_instr (Sskip cont);
-                ret succ'
-            | locals :: _ =>
-                do drop_start <- add_endscope_list ce locals cont;
-                do succ' <- add_instr (Sskip drop_start);
-                ret succ'
-            end
-        end
-    | RustlightBase.Scall p a al =>
-        do succ' <- add_instr (Scall p a al succ);
-        ret succ'
-    | RustlightBase.Sreturn e =>
-        do n1 <- add_instr (Sreturn e);
-        let locals := concat live_vars in        
-        do n2 <- add_endscope_list ce locals n1;
-        do n3 <- add_instr (Sskip n2);
-        ret n3
-    end.
+(* [vars] is a stack of variable list. Eack stack frame corresponds to
+a loop where these variables are declared *)
+Fixpoint transl_stmt (stmt: RustlightBase.statement) (vars: list (list (ident * type))) : statement :=
+  match stmt with
+  | RustlightBase.Sskip => Sskip
+  | Slet id ty stmt' =>
+      let s := transl_stmt stmt' (list_list_cons (id,ty) vars) in
+      let drop := Sdrop (Plocal id ty) in
+      Ssequence (Sstoragelive id) (Ssequence s (Ssequence drop (Sstoragedead id)))
+  | RustlightBase.Sassign p be =>
+      Sassign p be
+  | RustlightBase.Scall p e el =>
+      Scall p e el
+  | RustlightBase.Ssequence s1 s2 =>
+      let s1' := transl_stmt s1 vars in
+      let s2' := transl_stmt s2 vars in
+      Ssequence s1' s2'
+  | RustlightBase.Sifthenelse e s1 s2 =>
+      let s1' := transl_stmt s1 vars in
+      let s2' := transl_stmt s2 vars in
+      Sifthenelse e s1' s2'
+  | RustlightBase.Sloop s =>
+      let s := transl_stmt s (nil :: vars) in
+      Sloop s        
+  | RustlightBase.Sbreak =>
+      let drops := gen_drops (hd nil vars) in
+      Ssequence drops Sbreak
+  | RustlightBase.Scontinue =>
+      let drops := gen_drops (hd nil vars) in
+      Ssequence drops Scontinue
+  | RustlightBase.Sreturn e =>
+      Sreturn e
+  end.
+
 
 
 Fixpoint extract_vars (stmt: RustlightBase.statement) : list (ident * type) :=
   match stmt with
-  | Slet id ty _ s =>
+  | Slet id ty s =>
       (id,ty) :: extract_vars s
-  | Ssequence s1 s2 =>
+  | RustlightBase.Ssequence s1 s2 =>
       extract_vars s1 ++ extract_vars s2
   | RustlightBase.Sifthenelse _ s1 s2 =>
       extract_vars s1 ++ extract_vars s2
-  | Sloop s =>
+  | RustlightBase.Sloop s =>
       extract_vars s
   | _ => nil
   end.
 
-(** Translation of function  *)
 
-(* return the entry block and the temporary variables *)
-Definition transl_fun (f: RustlightBase.function) : mon node :=
-  (* add this return statement in case of there is no return in f *)
-  do return_node <- add_instr (Sreturn None);
-  (* add drops for the function parameter in return_block *)
-  do drop_start <- add_endscope_list ce f.(RustlightBase.fn_params) return_node;
-  do entry <- transl_stmt f.(RustlightBase.fn_body) drop_start (f.(RustlightBase.fn_params) :: nil) None None;
-  (* add storagelive for parameters *)
-  do entry' <- fold_right (fun elt acc => do n <- acc; add_instr (Sstoragelive (fst elt) n)) (ret entry) f.(RustlightBase.fn_params);
-  ret entry'.
-
-
-Definition transl_function (f: RustlightBase.function) : Errors.res function :=
+(* The main job is to extract the variables and translate the statement *)
+Definition transl_function (f: RustlightBase.function) : function :=
   let vars := extract_vars f.(RustlightBase.fn_body) in
-  let init_state := init_state in
-  match transl_fun f init_state with
-  | Error msg => Errors.Error msg
-  | OK entry s i =>
-      Errors.OK (Build_function
-                   f.(RustlightBase.fn_return)
-                   f.(RustlightBase.fn_callconv)
-                   f.(RustlightBase.fn_params)
-                   vars
-                   nil
-                   s.(st_code)
-                  entry)
-  end.
+  mkfunction f.(RustlightBase.fn_return)
+             f.(RustlightBase.fn_callconv)
+             f.(RustlightBase.fn_params)
+             vars
+             (transl_stmt f.(RustlightBase.fn_body) nil).
 
-Global Open Scope error_monad_scope.
-
-Definition transl_fundef (fd: RustlightBase.fundef) : Errors.res fundef :=
+Definition transl_fundef (fd: RustlightBase.fundef) : fundef :=
   match fd with
-  | Internal f => do tf <- transl_function f; Errors.OK (Internal tf)
-  | External _ ef targs tres cconv => Errors.OK (External function ef targs tres cconv)
+  | Internal f => (Internal (transl_function f))
+  | External _ ef targs tres cconv => External function ef targs tres cconv
   end.
 
-End COMPOSITE_ENV.
-
-
-(** Translation of a whole program. *)
-
-Definition transl_program (p: RustlightBase.program) : Errors.res RustIR.program :=
-  do p1 <- transform_partial_program (transl_fundef p.(prog_comp_env)) p;
-  Errors.OK {| prog_defs := AST.prog_defs p1;
-        prog_public := AST.prog_public p1;
-        prog_main := AST.prog_main p1;
-        prog_types := prog_types p;
-        prog_comp_env := prog_comp_env p;
-        prog_comp_env_eq := prog_comp_env_eq p |}.
+Definition transl_program (p: RustlightBase.program) : program :=
+  let p1 := transform_program transl_fundef p in
+  {| prog_defs := AST.prog_defs p1;
+    prog_public := AST.prog_public p1;
+    prog_main := AST.prog_main p1;
+    prog_types := prog_types p;
+    prog_comp_env := prog_comp_env p;
+    prog_comp_env_eq := prog_comp_env_eq p |}.
